added applicationwebsite translation, first draft

applicationwebsite.bpl
@@ -1,7 +1,80 @@
-var mapOfAvailableColleges:[Ref]MapIntCollege;
+var mapOfAvailableColleges : [Ref]MapIntCollege;
 
-var packedApplicationWebsiteField:[Ref]bool;
-var fracApplicationWebsiteField:[Ref]real;
+var packedApplicationWebsiteField : [Ref]bool;
+var fracApplicationWebsiteField : [Ref]real;
+
+procedure PackApplicationWebsiteField(m: MapIntCollege, this:Ref);
+requires (packedApplicationWebsiteField[this]==false) &&
+ 	(mapOfAvailableColleges[this] == m); 
+
+procedure UnpackApplicationWebsiteField(m: MapIntCollege, this:Ref);
+requires packedApplicationWebsiteField[this];
+ensures	(mapOfAvailableColleges[this] == m); 
+
+procedure submitApplicationGetCollege(int collegeNumber) returns (r: Ref)
+// TODO add modifies
+requires packedApplicationWebsiteField[this] && 
+	(fracApplicationWebsiteField[this] > 0.0);
+
+ensures ( packedCollegeBuildingsFew[result] && 
+	(fracCollegeBuildingsFew[result] > 0.0) ) ||
+	( packedCollegeBuildingsMany[result] &&
+	(fracCollegeBuildingsMany[result] > 0.0) );
+{
+	var college : Ref;
+	call college := lookup(collegeNumber, mapOfAvailableColleges[this]);
+	// might be able to say var r : Ref from the beginning
+	r := college;
+}
+
+procedure main(this:Ref) 
+// TODO add modifies
+{
+	var website : Ref;
+	var college, college2 : Ref;
+	var app1, app2 : Ref;
+	var app3, app4 : Ref;
+	assume (college != college2);
+	assume (app1 != app2);
+	assume (app3 != app4);
+	
+	call ConstructApplicationWebsite(website);
+	// TODO add the right statements after this constructor
+	// ApplicationWebsite website = new ApplicationWebsite()();
+
+	call college := submitApplicationGetCollege(2, website);
+
+	call ConstructStudentApplication(college, 3, app1);
+	//TODO write the needed statements after this constructor
+	// StudentApplication app1 = new StudentApplication(StudentAppFacilitiesFew())(college, 3);
+
+	call ConstructStudentApplication(college, 2, app2);
+	// TODO write after constructor
+	// StudentApplication app2 = new StudentApplication(StudentAppFacilitiesFew())(college, 2);
+
+	call checkFewFacilities(app1);
+	call changeApplicationFew(34, app1);
+	call checkFewFacilities(app2);
+
+	// ---- code below this is similar to above
+
+	call college2 := submitApplicationGetCollege(56, website);
+
+	call ConstructStudentApplication(college2, 45, app3);
+	//TODO write the needed statements after this constructor
+	// StudentApplication app3 = new StudentApplication(StudentAppFacilitiesMany())(college2, 45);
+
+	call ConstructStudentApplication(college2, 97, app4);
+	// TODO write after constructor
+	// StudentApplication app4 = new StudentApplication(StudentAppFacilitiesMany())(college2, 97);
+
+	call checkFewFacilities(app3);
+	call changeApplicationFew(78, app3);
+	call checkFewFacilities(app4);
+}
+
+
+
 
 
 
